UTerminator.Wf.allEq

FreydSSA/Terminator/Extrinsic/Basic.lean
@@ -2,7 +2,7 @@ import FreydSSA.Term.Extrinsic.Basic
 
 variable {φ ν α} [Φ : InstSet φ (Ty α)] [Φc : CohInstSet φ (Ty α)]
 
-inductive UTerminator.Wf : Ctx ν (Ty α) → UTerminator φ ν κ → LCtx ν (Ty α) κ → Type _
+inductive UTerminator.Wf : Ctx ν (Ty α) → UTerminator φ ν κ → LCtx ν κ (Ty α) → Type _
   | br : LCtx.Wk [⟨ℓ, A, Γ⟩] L → e.Wf 1 Γ A → Wf Γ (br ℓ e) L
   | ite : c.Wf 1 Γ Ty.bool → t.Wf Γ L → f.Wf Γ L → Wf Γ (ite c t f) L
 
@@ -15,10 +15,25 @@ def UTerminator.Wf.wk_entry {Γ Δ : Ctx ν (Ty α)} {t : UTerminator φ ν κ} 
   | br hℓ e => br ((w.to_lctx _ _).comp hℓ) (e.wk w)
   | ite c t f => ite (c.wk w) (t.wk_entry w) (f.wk_entry w)
 
-def UTerminator.Wf.wk_exit {L K : LCtx ν (Ty α) κ} {t : UTerminator φ ν κ}
+def UTerminator.Wf.wk_exit {L K : LCtx ν κ (Ty α)} {t : UTerminator φ ν κ}
   : Wf Γ t L → L.Wk K → Wf Γ t K
   | br hℓ e, w => br (hℓ.comp w) e
   | ite c t f, w => ite c (t.wk_exit w) (f.wk_exit w)
+
+theorem UTerminator.Wf.allEq {Γ : Ctx ν (Ty α)} {t : UTerminator φ ν κ}
+  (dt : Wf Γ t L) (dt' : Wf Γ t L) : dt = dt'
+  := by
+  induction dt <;> cases dt'
+  case br.br de _ de' _ =>
+    cases de.tyEq de'
+    congr
+    apply LCtx.Wk.allEq
+    apply de.allEq
+  case ite.ite =>
+    congr
+    apply UTm.Wf.allEq
+    apply_assumption
+    apply_assumption
 
 --TODO: Wf.toUGRegion
 
